Added new definitions and cool theorems

players/Hannah.lean
@@ -7,17 +7,12 @@ inductive ListNat where
 
 
 open ListNat -- Easier to write ListNat things
+open Nat
 
 #check nil -- With open command
 #check ListNat.nil -- Without "open ListNat" command
 #check cons 0 nil
 #eval nil -- deriving Repr
-
-
-
-
-
-
 
 
 -- LEVEL 2: Defining operations
@@ -30,13 +25,244 @@ def length : ListNat → Nat
 #eval length nil -- Evaluation (?)
 #eval length (cons 0 nil) -- Fix it
 
-def greatest : ListNat → Nat 
-  | nil => 0
-  | cons n l => if n > greatest l then n else greatest l
+def elem : Nat → ListNat → Bool
+  | _, nil => false
+  | n, (cons m l) => n == m || elem n l
 
-#eval greatest nil
-#eval greatest (cons 4 (cons 20 (cons 10 nil)))
-#eval greatest (cons 1 (cons 1 nil))
+#eval elem 8 nil
+#eval elem 5 (cons 4 (cons 6 (cons 5 nil)))
+
+def sum : ListNat → Nat
+  | nil => 0
+  | cons n l => n + (sum l)  
+
+#eval sum nil
+#eval sum (cons 3 (cons 5 (cons 8 nil)))
+
+def product : ListNat → Nat
+  | nil => 1
+  | cons n l => n * (product l)
+
+#eval product nil
+#eval product (cons 3 (cons 2 nil))
+
+-- Same as (++)
+def concat : ListNat → ListNat → ListNat
+  | nil, list => list
+  | (cons n l), list => cons n (concat l list)
+
+#eval concat nil nil
+#eval concat (cons 1 nil) (cons 3 (cons 4 nil))
+
+-- Add an nat to the end
+def append : Nat → ListNat → ListNat
+  | n, nil => cons n nil
+  | n, cons m l => cons m (append n l)
+
+-- Define append in function of concat
+
+def append_cat : Nat → ListNat → ListNat
+  | n, list => concat list (cons n nil)
+
+#eval append 0 nil
+#eval append 3 (cons 0 (cons 4 nil))
+
+-- esreveR...
+def reverse : ListNat → ListNat
+  | nil => nil
+  | cons n l => append n (reverse l)
+
+#eval reverse (cons 0 nil)
+#eval reverse (cons 1 (cons 3 (cons 4 nil)))
+
+def min₂ : Nat → Nat → Nat
+  | n+1, m+1 => (min n m) + 1
+  | _, _ => 0
+
+#eval min₂ 0 1
+#eval min₂ 5 9
+
+def max₂ : Nat → Nat → Nat
+  | 0, m => m
+  | n, 0 => n
+  | n+1, m+1 => (max n m) + 1
+
+#eval max₂ 0 1
+#eval max₂ 9 7
+
+def filter : (Nat → Bool) → ListNat → ListNat
+  | _, nil => nil
+  | p, cons n l => if p n then cons n (filter p l) else filter p l
+
+def even : Nat → Bool
+  | 0 => true
+  | succ 0 => false
+  | succ (succ n) => even n
+ 
+#eval filter even nil
+#eval filter even (cons 0 (cons 2 (cons 3 nil)))
+
+def odd : Nat → Bool
+  | 0 => false
+  | succ 0 => true
+  | succ (succ n) => odd n
+
+#eval odd 4
+#eval odd 7
+
+def Zero : Nat → Bool
+  | 0 => true
+  | _ => false
+
+#eval Zero 1
+#eval Zero zero
+
+def all : (Nat → Bool) → ListNat → Bool
+  | _, nil => true
+  | p, cons n l => p n && all p l
+
+#eval all even (cons 8 (cons 4 (cons 6 nil)))
+#eval all even (cons 2 (cons 6 (cons 7 nil)))
+#eval all odd (cons 5 (cons 2 (cons 7 (cons 9 nil))))
+#eval all odd nil
+#eval all Zero (cons 0 (cons 0 (cons 0 (cons 0 nil))))
+#eval all Zero (cons 0 (cons 1 (cons 0 (cons 6 nil))))
+
+
+def any : (Nat → Bool) → ListNat → Bool
+  | _, nil => false
+  | p, cons n l => p n || any p l
+
+#eval any even (cons 2 (cons 6 (cons 7 nil)))
+#eval any even (cons 5 (cons 7 (cons 9 (cons 3 nil))))
+#eval any odd (cons 6 (cons 4 (cons 2 (cons 1 nil))))
+#eval any odd (cons 4 nil)
+#eval any Zero (cons 7 (cons 5 (cons 1 (cons 6 nil))))
+#eval any Zero (cons 5 (cons 6 (cons 8 (cons 0 nil))))
+
+-- [1,2,3] → [2,4,6]
+def doubleList : ListNat → ListNat
+  | nil => nil
+  | cons n l => cons (n*2) (doubleList l)
+
+#eval doubleList nil
+#eval doubleList (cons 1 (cons 3 nil))
+
+def map : (Nat → Nat) → ListNat → ListNat
+  | _, nil => nil
+  | p, cons n l => cons (p n) (map p l)
+
+-- Use \. + space to write · 
+#eval map (· * 2) (cons 1 (cons 3 nil))
+#eval map (· + 3) (cons 1 nil)
+
+def addNat : Nat → ListNat → ListNat
+  | n, l => map (· + n) l
+
+#eval addNat 4 nil
+#eval addNat 8 (cons 0 (cons 5 (cons 1 nil)))
+
+def multNat : Nat → ListNat → ListNat
+  | n, l => map (· * n) l
+
+#eval multNat 3 (cons 1 (cons 2 (cons 3 nil)))
+#eval multNat 2 nil
+
+def expNat : Nat → ListNat → ListNat
+  | n, l => map (· ^ n) l
+
+#eval expNat 2 (cons 5 (cons 7 (cons 2 (cons 1 nil))))
+#eval expNat 3 nil
+
+def enumTo : Nat → ListNat
+  | n+1 => append (n+1) (enumTo n)
+  | _ => cons 0 nil
+
+#eval enumTo 3
+#eval enumTo 0
+
+def take : Nat → ListNat → ListNat
+  | n+1, (cons m l) => cons m (take n l)
+  | _, _ => nil
+
+#eval take 4 (cons 3 (cons 4 (cons 2 (cons 1 nil))))
+#eval take 6 (cons 3 (cons 3 nil))
+
+def drop : Nat → ListNat → ListNat
+  | n+1, (cons _ l) => drop n l
+  | _, l => l
+
+#eval drop 2 (cons 3 (cons 4 (cons 2 (cons 1 nil))))
+#eval drop 4 (cons 3 (cons 3 nil))
+
+def elemIndices : Nat → ListNat → ListNat
+  | n, cons m l => if n == m then cons 0 (addNat 1 (elemIndices n l)) else (addNat 1 (elemIndices n l))
+  | _, nil => nil
+
+#eval elemIndices 1 (cons 1 (cons 1 (cons 1 (cons 2 nil))))
+#eval elemIndices 3 (cons 2 (cons 1 (cons 0 (cons 9 nil))))
+
+def pwAdd : ListNat → ListNat → ListNat
+  | (cons n ns), (cons m ms) => cons (n+m) (pwAdd ns ms)
+  | _, _ => nil
+
+#eval pwAdd (cons 2 (cons 4 (cons 5 nil))) (cons 5 (cons 6 nil))
+#eval pwAdd (cons 1 (cons 2 nil)) (cons 6 (cons 5 (cons 4 nil)))
+
+def pwMult : ListNat → ListNat → ListNat
+  | (cons n ns), (cons m ms) => cons (n*m) (pwMult ns ms)
+  | _, _ => nil
+
+#eval pwMult (cons 2 (cons 4 (cons 5 nil))) (cons 5 (cons 6 nil))
+#eval pwMult (cons 1 (cons 2 nil)) (cons 6 (cons 5 (cons 4 nil)))
+
+def isSorted : ListNat → Bool
+  | cons n (cons m l) => n ≤ m && isSorted l
+  | _ => true
+
+#eval isSorted (cons 3 (cons 2 nil))
+#eval isSorted (cons 1 (cons 2 (cons 3 (cons 4 nil))))
+
+def minimum : ListNat → Nat
+  | cons n nil => n
+  | cons n l => min₂ n (minimum l)
+  | _ => 100000000000-- Error (to be fixed)
+
+#eval minimum (cons 3 (cons 5 (cons 1 (cons 8 nil))))
+#eval minimum (cons 4 nil)
+
+def maximum : ListNat → Nat 
+  | nil => 0
+  | cons n l => max₂ n (maximum l)
+
+#eval maximum nil
+#eval maximum (cons 10 (cons 5 (cons 7 nil)))
+#eval maximum (cons 1 (cons 1 nil))
+
+def isPrefixOf : ListNat → ListNat → Bool
+  | nil, _ => true
+  | cons n ns, cons m ms => n == m && isPrefixOf ns ms
+  | _, _ => false
+
+#eval isPrefixOf (cons 1 (cons 2 (cons 3 nil))) (cons 1 (cons 2 (cons 3 (cons 4 nil))))
+#eval isPrefixOf (cons 3 nil) (cons 2 nil)
+#eval isPrefixOf (cons 7 nil) nil
+
+def mix : ListNat → ListNat → ListNat
+  | cons n ns, cons m ms => (cons n (cons m (mix ns ms)))
+  | _, _ => nil
+
+#eval mix (cons 1 (cons 2 nil)) (cons 10 (cons 20 (cons 30 nil)))
+#eval mix nil (cons 3 nil)
+
+def interspace : Nat → ListNat → ListNat
+  | _, cons m nil => cons m nil
+  | n, cons m l => (cons m (cons n (interspace n l)))
+  | _, nil => nil
+
+#eval interspace 4 (cons 7 nil)
+#eval interspace 5 (cons 10 (cons 20 (cons 30 nil)))
+#eval interspace 7 nil
 
 -- Assume ordered lists
 -- First element greater than n
@@ -57,67 +283,6 @@ def lower_bound : Nat → ListNat → Nat
 #eval lower_bound 0 nil
 #eval lower_bound 3 (cons 1 (cons 3 (cons 4 (cons 8 nil))))
 #eval lower_bound 5 (cons 1 (cons 3 (cons 4 (cons 8 nil))))
-
-def filter : (Nat → Bool) → ListNat → ListNat
-  | _, nil => nil
-  | function, cons n l => if function n = True then cons n (filter function l) else filter function l
-open Nat
-
-def even : Nat → Bool
-  | 0 => True
-  | 1 => False
-  | n+2 => even n
- 
-#eval filter even nil
-#eval filter even (cons 0 (cons 2 (cons 3 nil)))
-
--- [1,2,3] → [2,4,6]
-def doubleList : ListNat → ListNat
-  | nil => nil
-  | cons n l => cons (n*2) (doubleList l)
-
-def map : (Nat → Nat) → ListNat → ListNat
-  | _, nil => nil
-  | function, cons n l => cons (function n) (map function l)
-
-#eval doubleList nil
-#eval doubleList (cons 1 (cons 3 nil))
-
--- Use \. + space to write · 
-#eval map (· * 2) (cons 1 (cons 3 nil))
-#eval map (· + 3) (cons 1 nil)
-
-
-def concat : ListNat → ListNat → ListNat
-  | nil, list => list
-  | (cons n l), list => cons n (concat l list)
-
-#eval concat nil nil
-#eval concat (cons 1 nil) (cons 3 (cons 4 nil))
--- Yours!
-
--- Add an nat to the end
-def append : Nat → ListNat → ListNat
-  | n, nil => cons n nil
-  | n, cons m l => cons m (append n l)
-
--- Define append in function of concat
-
-def append_cat : Nat → ListNat → ListNat
-  | n, list => concat list (cons n nil)
-
-#eval append 0 nil
-#eval append 3 (cons 0 (cons 4 nil))
-
--- esreveR...
-def reverse : ListNat → ListNat
-  | nil => nil
-  | cons n l => append n (reverse l)
-
--- Obviously eval it...
-
-#eval reverse (cons 0 nil)
-#eval reverse (cons 1 (cons 3 (cons 4 nil)))
 
 -- LEVEL 3: Theorems
 
@@ -150,18 +315,86 @@ by
   | cons n l' h => rw [reverse, cool_theorem (reverse l') n, h]
 
 
-
-
-
-
-
-
-
 -- LEVEL 4: Your own theorems
 
--- Sugestions:
--- Can you think cool theorems about lower_bound and upper_bound?
--- How about append_cat?
--- Buy me a KitKat
+-- HW Theorems
 
--- By Isaac Lourenço 2023, IMD - UFRN, Brazil.
+-- Level 4.1
+theorem sum_distr_concat (xs ys : ListNat) :
+  sum (concat xs ys) = sum xs + sum ys :=
+by
+  induction xs with
+  | nil => rw [concat, sum, Nat.zero_add]
+  | cons x xs h => rw [concat, sum, h, sum, Nat.add_assoc]
+
+-- Level 4.2
+theorem product_distr_concat (xs ys : ListNat) :
+  product (concat xs ys) = product xs * product ys :=
+by
+  induction xs with
+  | nil => rw [concat, product, Nat.one_mul]
+  | cons x xs h => rw [concat, product, h, product, Nat.mul_assoc]
+
+-- Level 4.3
+theorem le_succ_succ_self (n : Nat) :
+  n < succ (succ n) :=
+by
+  have h: (succ n < succ (succ n) ∨ succ n ≥ succ (succ n)) := Nat.lt_or_ge (succ n) (succ (succ n))
+  apply Or.elim h
+  intro h'
+  have h1: (n ≤ succ n) := Nat.le_succ n
+  exact Nat.lt_of_le_of_lt h1 h'
+  intro h2
+  have h_boom: (¬succ (succ n) ≤ succ n) := Nat.not_succ_le_self (succ n)
+  exact False.elim (h_boom h2)
+
+theorem odd_eq_not_even (n : Nat) :
+  odd n = not (even n) :=
+by
+  induction n using Nat.strongInductionOn with
+  | ind n ih =>
+    match n with
+    | 0 => rw [odd, even, Bool.not_true]
+    | succ 0 => rw [odd, even, Bool.not_false]
+    | succ (succ n') => 
+      rw [odd, even, ih n' (le_succ_succ_self n')]
+
+theorem length_concat_distr (xs ys : ListNat) :
+  length (concat xs ys) = length xs + length ys :=
+by
+  induction xs with
+  | nil => rw [concat, length, Nat.zero_add]
+  | cons x xs h => rw [concat, length, h, length, Nat.add_right_comm]
+
+theorem false_not_true :
+  false ≠ true :=
+by
+  intro H
+  cases H
+
+theorem length_concat_filter_even_odd_list (l : ListNat):
+  length (concat (filter even l) (filter odd l)) = length l :=
+by
+  induction l with
+  | nil => rw [filter, filter, concat]
+  | cons x xs h => 
+    rw [filter, filter, odd_eq_not_even]
+    cases even x
+    rw [Bool.not_false,
+        if_neg false_not_true,
+        if_pos rfl,
+        length,
+        length_concat_distr,
+        length,
+        ← Nat.add_assoc, 
+        ← length_concat_distr,
+        h]
+    rw [if_pos rfl,
+        Bool.not_true,
+        if_neg false_not_true,
+        concat, 
+        length,
+        length_concat_distr,
+        length,
+        ← length_concat_distr,
+        h]
